# Kompleksna stevila
### 2. vaja
$$w = (5+2i)^2 + (1 - 2i)^2 -(4+3i)(3-2i) + \frac{13(1-i)}{2+3i} - i^{23} + 5- 14i$$
$$(5+2i)^2 = 25 +20i -4 = 21 + 20 i$$
$$(1-2i)^2 = 1 -4i -4 = -3 -4i$$
$$(4+3i)(3-2i) = 12 -8i + 9i +6 = 18 + i$$
$$\frac{13(1-i)}{2+3i} = \frac{13(1-i)(2-3i)}{(2+3i)(2-3i)} = \frac{13(2-3i-2i-3)}{4+9} = -1 -5i$$
$$i^{23} = i^{5 \cdot 4 + 3 } = i^3 = -i$$
$$w = 21 + 20i -3 -4i -18 -i -1 -5i + i + 5 -14i = -4 -3i$$
$$w = -4 -3i$$
$Re(w) = -4$
$Im(w) = -3$
$\overline w = -4 + 3i$
$|w| = \sqrt{(-4)^2 + (-3)} = \sqrt{16 + 9} = \sqrt{25} = 5$

### 3. vaja
$$f(x) = \sqrt{x^2 -4x + 3}$$
$$D_f = ? $$
$$x^2 - 4x +3 >= 0$$
$$x_{1,2} = \frac{4 \pm \sqrt{16 - 4 \cdot 3}}{2} = \frac{4 \pm \sqrt{4}}{2} = 2 \pm 1$$
$$x_1 = 3, x_2 = 1$$
$$D_f = (-\infty, 1] U [3, \infty)$$

### 4. naloga
$$f(x) = \ln\frac{x-1}{2x+7} + \sqrt{x^2 -4} $$
$$\ln\frac{x-1}{2x+7} $$
$$\frac{x-1}{2x+7} > 0$$
$$(-\infty, -3.5) U (1, \infty)$$
$$x^2 -4 >= 0 $$
$$(-\infty, -2]U[2, \infty)$$
$$D_f = (-\infty,â€”3.5) U [2, \infty)$$
### 8. naloga
$$3x + 2y - 13 = 0, 7x -4y -13 = 0, T(2, -3)$$
$$6x + 4y -26 = 0,
  7x - 4y -13 = 0 \Rightarrow
  13x - 3 \cdot 13 = 0 \Rightarrow
  13x = 3 \cdot 13 \Rightarrow
  x = 3
$$
$$3 \cdot 3 + 2y - 13 = 0 \Rightarrow 2y = 4 \Rightarrow y = 2$$
$$P(3, 2), T(2, -3)$$
$$ k = \frac{-3 -2}{2 -3} = \frac {-5} {-1}$$







### 10. naloga
$$x_1=-1, A(0, -1), B(1, 4)$$
$$a(x+1)(x-x_2) =y$$
$$a(0+1)(0-x_2) =-1 \Rightarrow -x_2 \cdot a = -1 \Rightarrow a = \frac{-1}{-x_2} \Rightarrow a = x_2^{-1}$$
$$a(1+1)(1-x_2) =4 \Rightarrow a(1-x_2) = 2$$
$$ \frac{1}{x_2} = \frac{2}{1-x_2}$$
$$1-x_2 = 2x_2 \Rightarrow x_2 = \frac 1 3$$
$$a = 3$$
$$y = 3(x+1)(x-\frac 1 3), y = 3(x^2 - \frac x 3 + x -\frac 1 3) = 3x^2 - x + 3x - 1 = 3x^2 + 2x -1$$

$$3x^2 + 2x -1 = 3 (x^2 + \frac 2 3 x) - 1 = 3((x-\frac 1 3)^2 - \frac 1 9) -1
$$


### 11. naloga
$$ f(x) = 2x^2 +(t + 5)x + 8$$
$$D = (t+5)^2 -4 \cdot 2 \cdot 8 = 0 $$
$$t^2 + 10 t + 25 - 64 =0$$
$$t^2 + 10t - 39 = 0$$
$$t_{1, 2} = \frac{-10 \pm \sqrt{100 + 4\cdot 39}}{}$$

### 12. naloga
$$e^{\ln \frac 1 3} + \log_4 4^5 + \log_2 \frac 1 {\sqrt[3]{16}} = \frac 1 3 + 5 $$


### 13. naloga
#### A
$$5^{x+1} - 3^x = 3^{x+1} + 5^x$$
$$5^x(5-1) = 3^x(3+1)$$
$$5^x = 3^x$$
$$x = 0$$
B
$$5^x + 2^{1-x} \cdot 10 ^x = 375$$
$$5^x + 2^{1-x} \cdot 2 ^x \cdot 5^x = 375$$

C
$$\log(x) + \log(x-3) = 2 \log(6 - x) = \log(x^2 - 3x)$$
$$ 2 = \frac{\log(x^2 - 3x)}{\log(6 - x)} = \log(x^2 - 2x - 6) $$
$$10^2 = x^2 -2x -6$$
$$x^2 -2x - 106 = 0$$




# Kotne funkcije
3. naloga
A
$$\sin(x+\frac \pi 2) = - \frac 1 2$$
$$x + \frac \pi 2 = \frac 7 6 \pi + 2k\pi; k = Z$$

$$x + \frac \pi 2 = - \frac 1 6 \pi + 2k\pi; k = Z$$

B
$$\sin^2 x - \cos^2x = \frac 1 2$$
$$-\sin^2 x + \cos^2x = -\frac 1 2$$
$$\cos(2x) = -\frac 1 2$$
$$2x_{1,2}  = \pm \frac 2 3 \pi + 2k\pi;k = Z$$
$$x_{1,2}  = \pm \frac 1 3 \pi + k\pi;k = Z$$
2. naloga
A
$$(\sin(\alpha) + \cos(\alpha))^2 = 1 + \sin(2\alpha)$$

$$\sin^2(\alpha) + \cos^2(\alpha) + 2\sin(\alpha)\cos(\alpha) = 1 + 2\sin(\alpha)\cos(\alpha)$$
